sorry, no(t) sorry

theories/Borda_Rule_Ref.thy
@@ -4,29 +4,8 @@ theory Borda_Rule_Ref
           "Compositional_Structures/Elect_Composition_Ref"              
 begin
 
-definition borda_rule_sep where
-  "borda_rule_sep \<equiv> elector_sep borda_elim_sep"
 
-                          
-interpretation borda_rule_impl: elector_sepref borda_ref borda_elim_sep borda
-  apply unfold_locales            
-  subgoal using borda_elim_sep.refine .
-  subgoal using borda_sound .
-  subgoal apply (intro frefI) using borda_ref_correct[THEN frefD] by auto
-  done
 
-thm "borda_rule_impl.elector_sep_correct"
-
-lemma  borda_rule_correct:
-  shows "(uncurry borda_rule_sep, uncurry (RETURN oo borda_rule))
-    \<in> [\<lambda>(a, b).
-           finite_profile a b]\<^sub>a (alts_set_impl_assn id_assn)\<^sup>k *\<^sub>a
-                 (list_assn
-                   (hr_comp (ballot_impl_assn id_assn)
-                     ballot_rel))\<^sup>k \<rightarrow> result_impl_assn id_assn"
-  unfolding borda_rule_sep_def borda_rule.simps 
-  using borda_rule_impl.elector_sep_correct unfolding in_br_conv well_formed_pl_def
-  .
 sepref_definition borda_rule_sep_direct is "uncurry (seq_opt borda elect_module
   )"
   :: "[\<lambda>(x, xa).
@@ -72,7 +51,8 @@ lemma borda_rule_opt_direct_correct:
   by (metis)
   
 
-export_code convert_list_to_hash_set clist borda_rule_opt_sep_direct in Scala_imp
+export_code convert_list_to_hash_set clist borda_rule_opt_sep_direct in Scala_imp 
 
+export_code convert_list_to_hash_set clist borda_rule_sep_direct in Scala_imp 
                                           
 end
