theories/Compositional_Structures/Elect_Composition_Ref.thy
@@ -4,10 +4,6 @@ theory Elect_Composition_Ref
           Sequential_Composition_Ref
 begin
 
-
-definition  
-  "elector_sep m \<equiv> m \<triangleright>sep elect_module_sep"
-
 definition elector_opt :: "('a set \<Rightarrow> 'a Profile \<Rightarrow> 'a Result nres) \<Rightarrow> 
   'a set \<Rightarrow> 'a Profile \<Rightarrow> 'a Result nres" where
   "elector_opt m A p \<equiv> do { 
@@ -50,57 +46,6 @@ proof (rename_tac A p, refine_vcg, unfold SPEC_eq_is_RETURN)
                         \<le> RETURN (elect m A p \<union> defer m A p, reject m A p, {}))"
     by (simp add: case_prod_beta' order_trans)
 qed
-    
-
-thm "elector_sep_def"
-
-locale elector_impl =  
-  fixes m_ref :: "'a::{default, hashable, heap} Electoral_Module_Ref"
-  fixes m_sep :: "('a::{default, hashable, heap}, unit) hashtable
-      \<Rightarrow> ('a::{default, hashable, heap} array \<times> nat) list
-         \<Rightarrow> (('a::{default, hashable, heap}, unit) hashtable
-   \<times> ('a::{default, hashable, heap}, unit) hashtable \<times> ('a::{default, hashable, heap}, unit) hashtable) Heap"
-  assumes 
-    m_impl: "(uncurry m_sep, uncurry m_ref)
-        \<in> (alts_set_impl_assn id_assn)\<^sup>k *\<^sub>a (profile_impl_assn id_assn)\<^sup>k 
-      \<rightarrow>\<^sub>a result_impl_assn id_assn"
-
-
-locale elector_sepref = elector_impl +
-  fixes m :: "'a::{default, hashable, heap}  Electoral_Module"
-assumes module_m: "electoral_module m"
-assumes m_ref_correct: "(uncurry m_ref, uncurry (RETURN oo m)) \<in> 
-  ([\<lambda> (A, pl). finite_profile A
-            pl]\<^sub>f (\<langle>Id\<rangle>set_rel \<times>\<^sub>r profile_rel)
-   \<rightarrow> \<langle>\<langle>Id\<rangle>set_rel \<times>\<^sub>r \<langle>Id\<rangle>set_rel \<times>\<^sub>r \<langle>Id\<rangle>set_rel\<rangle>nres_rel)" 
-begin
-
-interpretation elector: sequence_sepref m_ref m_sep elect_module_ref elect_module_sep m elect_module
-  apply unfold_locales
-  subgoal using m_impl .
-  subgoal  using elect_module_sep.refine .
-  subgoal using module_m.
-  subgoal by simp
-  subgoal using m_ref_correct.
-  subgoal apply (intro frefI nres_relI) 
-    using elect_module_ref_correct[THEN frefD, THEN nres_relD]
-    unfolding comp_apply by auto
-  done
-
-
-lemmas elector_sep_correct_aux =  elector.sequence_correct
-
-lemma elector_sep_correct:
-  shows "(uncurry (elector_sep m_sep), uncurry (RETURN oo elector m))
-      \<in> [\<lambda>(a, b).
-           finite_profile a b]\<^sub>a (alts_set_impl_assn id_assn)\<^sup>k *\<^sub>a
-                 (list_assn
-                   (hr_comp (ballot_impl_assn id_assn)
-                     ballot_rel))\<^sup>k \<rightarrow> result_impl_assn id_assn"                                               
-  unfolding elector_sep_def elector.simps 
-  using elector_sep_correct_aux by simp
-
-
-end
+   
 
 end
