theories/Pairwise_Majority_Rule_Ref.thy
@@ -4,43 +4,22 @@ theory Pairwise_Majority_Rule_Ref
           "Compositional_Structures/Elect_Composition_Ref"              
 begin
 
-(*definition pairwise_majority_rule_sep where
-  "pairwise_majority_rule_sep \<equiv> elector_sep condorcet_elim_sep"
 
-
-interpretation pairwise_majority_rule_impl: 
-    elector_sepref condorcet_ref condorcet_elim_sep condorcet
-  apply unfold_locales
-  subgoal using condorcet_elim_sep.refine .
-  subgoal using condorcet_sound .
-  subgoal apply (intro frefI) using condorcet_ref_correct[THEN frefD] by auto
-  done
-
-lemma  pairwise_majority_rule_correct:
-  shows "(uncurry pairwise_majority_rule_sep, uncurry (RETURN oo pairwise_majority_rule))
-   \<in> [\<lambda>(a, b).
-           finite_profile a b]\<^sub>a (alts_set_impl_assn id_assn)\<^sup>k *\<^sub>a
-                 (list_assn
-                   (hr_comp (ballot_impl_assn id_assn)
-                     ballot_rel))\<^sup>k \<rightarrow> result_impl_assn id_assn"
-  unfolding pairwise_majority_rule_sep_def pairwise_majority_rule.simps 
-    using pairwise_majority_rule_impl.elector_sep_correct . *)
-
-sepref_definition pairwise_majority_rule_direct is "uncurry (seq_opt condorcet elect_module
-  )"
+sepref_definition pairwise_majority_rule_direct is "uncurry (elector_opt (RETURN oo condorcet))"
   :: "elec_mod_sep_rel nat_assn"
-  unfolding seq_opt_def
+  unfolding elector_opt_def hs.fold_custom_empty
   apply sepref_dbg_keep
   done
 
-lemmas opt_seq_pmc = seq_opt_correct[OF condorcet_sound elect_mod_sound]
+lemmas opt_seq_pmc = elector_opt_correct[of condorcet]
 lemmas opt_seq_pmct_aux = pairwise_majority_rule_direct.refine[FCOMP opt_seq_pmc]
 
 lemma opt_pmc_correct:
-  shows "(uncurry pairwise_majority_rule_direct, uncurry (RETURN oo (pairwise_majority_rule:: (nat Electoral_Module))))
+  shows "(uncurry pairwise_majority_rule_direct, 
+          uncurry (RETURN oo (pairwise_majority_rule:: (nat Electoral_Module))))
   \<in> elec_mod_sep_rel nat_assn"
-  unfolding pairwise_majority_rule.simps elector.simps 
-  using  opt_seq_pmct_aux  prod_rel_id_simp set_rel_id hr_comp_Id2
+  unfolding pairwise_majority_rule.simps
+  using  condorcet_sound opt_seq_pmct_aux  prod_rel_id_simp set_rel_id hr_comp_Id2
   by metis
 
 declare opt_pmc_correct [sepref_fr_rules]
